imp_system/mem/MemTactics.v
@@ -1,0 +1,43 @@
+Require Import CRIS.
+Require Export ImpPrelude MemHeader MemA.
+
+Section mem.
+  Context `{!crisG Γ Σ α β τ _S _I, !concG, !memG}.
+
+  Local Definition state : Type := alist key Any.t.
+  Local Definition post (R_s R_t : Type) : Type := state * R_s → state * R_t → iProp Σ.
+  Local Definition rel : Type := ∀ R_s R_t : Type,
+    post R_s R_t → bool → bool → state * itree crisE R_s → state * itree crisE R_t → iProp Σ.
+
+  Context (fl_s fl_t : alist (option string) (Any.t → itree crisE Any.t)).
+  Context (Ist : alist key Any.t → alist key Any.t → iProp Σ).
+  Context (R_s R_t : Type).
+  Context (RR : post R_s R_t).
+  Context (ps pt : bool).
+  Context (st_src st_tgt : state).
+
+  Lemma wsim_mem_alloc (sz : Z) k_s k_t E1 E2 r g img_t msk_t scp_t :
+    alist_find (Some MemHdr.alloc) fl_t =
+      Some (SB.sandbox_body
+        (SModTr.trans_ktree sp_none
+          (true, wmask_all, MemA.scopes, (Some (to_fspec MemSpec.alloc), fbody_trivial)))) →
+    (msk_t MemHdr.alloc : bool) →
+    (0 <= 8 * sz < modulus_64)%Z →
+    (∀ blk,
+      ([∗ list] i ↦ v ∈ repeat Vundef (Z.to_nat sz), (blk, Z.of_nat i)%Z ↦ v) -∗
+      wsim fl_s fl_t Ist (E1, E2) r g R_s R_t RR ps true
+      (st_src, k_s)
+      (st_tgt, k_t (Vptr (blk, 0%Z))↑))
+    ⊢ wsim fl_s fl_t Ist (E1, E2) r g R_s R_t RR ps pt
+    (st_src, k_s)
+    (st_tgt, x <- (SB.sandbox img_t msk_t scp_t (trigger (Call MemHdr.alloc [Vint sz]↑)));; k_t x).
+  Proof.
+    intros Hin Hmsk Hsz.
+    iIntros "K".
+    inline_r. steps_r. force_r (Z.to_nat sz). forces_r. iSplit; eauto.
+    { rewrite Z2Nat.id //; try lia. iSplit; eauto. iSplit; eauto. iPureIntro; lia. }
+    steps_r. iDestruct "GRT" as "[[% [-> ↦]] ->]". iApply "K".
+    iApply (big_sepL_impl with "↦").
+    iIntros "!> % % %"; rewrite Z.add_0_l; iIntros "$".
+  Qed.
+End mem.
